axiomatic_expressions.v
@@ -48,7 +48,7 @@ Lemma ax_expr_weaken Γ δ P P' A Q Q' e :
   P ⊆{Γ} P' → (∀ ν, Q' ν ⊆{Γ} Q ν) →
   Γ\ δ\ A ⊨ₑ {{ P' }} e {{ Q' }} → Γ\ δ\ A ⊨ₑ {{ P }} e {{ Q }}.
 Proof.
-  intros HP HQ Hax Δ n ρ m τlr ????????.
+  intros HP HQ Hax Γ' Δ n ρ m τlr ??????????.
   apply ax_weaken with (ax_expr_cond ρ A) (ax_expr_post Q' τlr) n; auto.
   destruct 2; constructor; auto. apply HQ; eauto using indexes_valid_weaken.
 Qed.
@@ -64,7 +64,7 @@ Lemma ax_expr_frame_r Γ δ B A P Q e :
   Γ\ δ\ B ⊨ₑ {{ P }} e {{ λ ν, Q ν }} →
   Γ\ δ\ B ⊨ₑ {{ P ★ A }} e {{ λ ν, Q ν ★ A }}.
 Proof.
-  intros Hax Δ n ρ m τlr ?? Hlocks ???? (m1&m2&?&?&?&?).
+  intros Hax Γ' Δ n ρ m τlr ???? Hlocks ???? (m1&m2&?&?&?&?).
   destruct (cmap_erase_union_inv m m1 m2)
     as (m1'&m2'&->&?&->&->); simplify_mem_disjoint_hyps; auto.
   rewrite mem_locks_union in Hlocks by auto; decompose_empty.
@@ -86,12 +86,12 @@ Qed.
 Lemma ax_expr_exist_pre {A} Γ δ (B : assert K) (P : A → assert K) Q e :
   (∀ x, Γ\ δ\ B ⊨ₑ {{ P x }} e {{ Q }}) →
   Γ\ δ\ B ⊨ₑ {{ ∃ x, P x }} e {{ Q }}.
-Proof. intros Hax Δ n k m τlr HΓ Hd ????? [x Hpre]. by apply (Hax x). Qed.
+Proof. intros Hax Γ' Δ n k m τlr HΓ Hd ??????? [x Hpre]; by apply (Hax x). Qed.
 Lemma ax_expr_funframe_r Γ δ B A P Q e :
   Γ\ δ\ A ★ B ⊨ₑ {{ P }} e {{ λ ν, Q ν }} →
   Γ\ δ\ B ⊨ₑ {{ P ★ A }} e {{ λ ν, Q ν ★ A }}.
 Proof.
-  cut (∀ n Δ ρ k φ m τlr,
+  revert Γ. cut (∀ Γ n Δ ρ k φ m τlr,
     ✓ Γ → ✓{Δ}* ρ →
     ax_graph (ax_expr_cond ρ (A ★ B)) (ax_expr_post Q τlr) Γ δ Δ ρ n k φ m →
     (k = [] → ∀ mA,
@@ -102,16 +102,16 @@ Proof.
     (k ≠ [] →
       ax_graph (ax_expr_cond ρ B)
                (ax_expr_post (λ ν, Q ν ★ A)%A τlr) Γ δ Δ ρ n k φ m)).
-  { intros help Hax Δ n ρ m' τlr HΓ ? Hm ??? (mB&?&?&?&?&?)
+  { intros help Γ Hax Γ' Δ n ρ m' τlr ???? Hm ??? (mB&?&?&?&?&?)
       (m&mA&?&?&?&?); simplify_equality.
     destruct (cmap_erase_union_inv_r m' m mA)
       as (m''&->&?&->&?); simplify_mem_disjoint_hyps; auto.
     rewrite mem_locks_union in Hm by auto; decompose_empty.
-    refine (proj1 (help n Δ ρ [] (Expr e) m'' τlr _ _ _ ) _ mA _ _ _ _ _); auto.
+    refine (proj1 (help Γ' n Δ ρ [] (Expr e) m'' τlr _ _ _ ) _ mA _ _ _ _ _); auto.
     apply Hax; auto. exists (mA ∪ mB); split_ands; eauto.
     * rewrite mem_locks_union by auto. by apply empty_union_L.
     * exists mA mB; split_ands; auto. }
-  clear P. intros n.
+  clear P. intros Γ n.
   induction n as [[|n] IH] using lt_wf_ind; [repeat constructor|].
   intros Δ ρ k φ m τlr ??;
     inversion 1 as [|??? [ν ?????]|???? Hred Hstep]; subst.
@@ -189,15 +189,15 @@ Lemma ax_expr_base Γ δ A P Q e ν :
   P ⊆{Γ} (Q ν ∧ e ⇓ ν)%A →
   Γ\ δ\ A ⊨ₑ {{ P }} e {{ Q }}.
 Proof.
-  intros HPQ Δ n ρ m τlr HΓ ??? He Hm HA HP.
-  destruct (HPQ Γ Δ ρ n (cmap_erase m)) as [HQ (τlr'&?&?)]; auto.
+  intros HPQ Γ' Δ n ρ m τlr ?????? He Hm HA HP.
+  destruct (HPQ Γ' Δ ρ n (cmap_erase m)) as [HQ (τlr'&?&?)]; auto.
   assert (τlr' = τlr) by (by simplify_type_equality'); subst.
   cut (∀ Δ' e',
-    Δ ⇒ₘ Δ' → locks e' = ∅ → ⟦ e' ⟧ Γ ρ m = Some ν → (Γ,Δ',ρ.*2) ⊢ e' : τlr →
+    Δ ⇒ₘ Δ' → locks e' = ∅ → ⟦ e' ⟧ Γ' ρ m = Some ν → (Γ',Δ',ρ.*2) ⊢ e' : τlr →
     ax_graph (ax_expr_cond ρ A)
-      (ax_expr_post Q τlr) Γ δ Δ' ρ n [] (Expr e') m).
+      (ax_expr_post Q τlr) Γ' δ Δ' ρ n [] (Expr e') m).
   { intros help. apply (help Δ); rewrite <-1?expr_eval_erase; auto. }
-  assert (✓{Γ,Δ} (cmap_erase m)) by eauto.
+  assert (✓{Γ',Δ} (cmap_erase m)) by eauto.
   clear HPQ HP He. induction n as [[|n] IH] using lt_wf_ind; [by constructor |].
   intros Δ' e' ? He' Heval ?. destruct (decide (is_nf e')) as [Hnf|Hnf].
   { inversion Hnf; simplify_option_equality; typed_inversion_all.
@@ -205,7 +205,7 @@ Proof.
   apply ax_further_alt.
   intros Δ'' n''; inversion_clear 4 as [mA mf|]; simplify_equality'; split.
   { destruct (is_nf_is_redex e') as (E&e''&?&->); auto.
-    destruct (expr_eval_subst_ehstep Γ ρ (m ∪ mf ∪ mA) E e'' ν)
+    destruct (expr_eval_subst_ehstep Γ' ρ (m ∪ mf ∪ mA) E e'' ν)
       as (e2&?&?); auto; try solve_rcred.
     eapply expr_eval_subseteq with Δ'' m τlr;
       eauto using indexes_valid_weaken, @sep_union_subseteq_l_transitive,
@@ -214,10 +214,10 @@ Proof.
   apply (rcstep_focus_inv _ _ _ _ _ _ p); clear p; try done.
   * intros E e1 e2 m2 -> p ?.
     rewrite expr_eval_subst in Heval; destruct Heval as (ν'&?&?).
-    destruct (ectx_subst_typed_rev Γ Δ'' (ρ.*2) E e1 τlr)
+    destruct (ectx_subst_typed_rev Γ' Δ'' (ρ.*2) E e1 τlr)
       as (τlr''&?&?); eauto using expr_typed_weaken.
     rewrite ectx_subst_locks in He'; decompose_empty.
-    assert (⟦ e1 ⟧ Γ ρ (m ∪ mf ∪ mA) = Some ν').
+    assert (⟦ e1 ⟧ Γ' ρ (m ∪ mf ∪ mA) = Some ν').
     { eapply expr_eval_subseteq with Δ'' m τlr'';
         eauto using indexes_valid_weaken, @sep_union_subseteq_l_transitive,
         @sep_union_subseteq_l', expr_typed_weaken. }
@@ -247,20 +247,20 @@ Lemma ax_rtol Γ δ A P Q1 Q2 e :
   Γ\ δ\ A ⊨ₑ {{ P }} e {{ Q1 }} →
   Γ\ δ\ A ⊨ₑ {{ P }} .* e {{ Q2 }}.
 Proof.
-  intros HQ Hax Δ n ρ m [τ|] ??? He1e2 He ???; typed_inversion_all.
-  apply (ax_expr_compose_1 Γ δ A Q1 _ Δ DCRtoL e ρ n m (inr (TType τ.*))); auto.
+  intros HQ Hax Γ' Δ n ρ m [τ|] ????? He1e2 He ???; typed_inversion_all.
+  apply (ax_expr_compose_1 Γ' δ A Q1 _ Δ DCRtoL e ρ n m (inr (TType τ.*))); auto.
   { esolve_elem_of. }
   clear dependent m; intros Δ' n' Ω [|v] m ??????; typed_inversion_all.
   apply ax_further_alt.
   intros Δ'' n'' ????? Hframe; inversion_clear Hframe as [mA mf|];
     simplify_equality; simplify_mem_disjoint_hyps.
-  destruct (HQ v Γ Δ' ρ n' (cmap_erase m)) as (a'&?&HA);
+  destruct (HQ v Γ' Δ' ρ n' (cmap_erase m)) as (a'&?&HA);
     simpl; eauto 10 using indexes_valid_weaken.
-  destruct (HA Γ Δ'' n'' mA) as (τlr&?&?); clear HA; eauto.
+  destruct (HA Γ' Δ'' n'' mA) as (τlr&?&?); clear HA; eauto.
   { rewrite <-cmap_erase_disjoint_le; auto. }
   destruct τlr as [τ'|]; simplify_option_equality; typed_inversion_all.
   assert (TType τ' = TType τ); [|simplify_equality].
-  { apply typed_unique with (Γ,Δ'') a'; eauto using addr_typed_weaken. }
+  { apply typed_unique with (Γ',Δ'') a'; eauto using addr_typed_weaken. }
   assert (index_alive' (m ∪ mf ∪ mA) (addr_index a')).
   { apply cmap_subseteq_index_alive' with (mA ∪ cmap_erase m); auto.
     rewrite (sep_commutative _ mA) by auto.
@@ -279,8 +279,8 @@ Lemma ax_rofl Γ δ A P Q1 Q2 e :
   Γ\ δ\ A ⊨ₑ {{ P }} e {{ Q1 }} →
   Γ\ δ\ A ⊨ₑ {{ P }} & e {{ Q2 }}.
 Proof.
-  intros HQ Hax Δ n ρ m [τ|] ??? He1e2 He ???; typed_inversion_all.
-  apply (ax_expr_compose_1 Γ δ A Q1 _ Δ DCRofL e ρ n m (inl τ)); auto.
+  intros HQ Hax Γ' Δ n ρ m [τ|] ????? He1e2 He ???; typed_inversion_all.
+  apply (ax_expr_compose_1 Γ' δ A Q1 _ Δ DCRofL e ρ n m (inl τ)); auto.
   { esolve_elem_of. }
   clear dependent m; intros Δ' n' Ω [a|] m ??????; typed_inversion_all.
   apply ax_further; [intros; solve_rcred|].
@@ -298,17 +298,17 @@ Lemma ax_load Γ δ A P Q1 Q2 e :
   Γ\ δ\ A ⊨ₑ {{ P }} e {{ Q1 }} →
   Γ\ δ\ A ⊨ₑ {{ P }} load e {{ Q2 }}.
 Proof.
-  intros HQ Hax Δ n ρ m [|τ] ?????? HA HP; typed_inversion_all.
-  apply (ax_expr_compose_1 Γ δ A Q1 _ Δ DCLoad e ρ n m (inl τ)); auto.
+  intros HQ Hax Γ' Δ n ρ m [|τ] ???????? HA HP; typed_inversion_all.
+  apply (ax_expr_compose_1 Γ' δ A Q1 _ Δ DCLoad e ρ n m (inl τ)); auto.
   { esolve_elem_of. }
   clear dependent m. intros Δ' n' Ω [a|] m ??????; typed_inversion_all.
   apply ax_further_alt; intros Δ'' n'' ????? Hframe;
     inversion_clear Hframe as [mA mf|]; simplify_equality.
-  destruct (HQ a Γ Δ' ρ n' (cmap_erase m))
+  destruct (HQ a Γ' Δ' ρ n' (cmap_erase m))
     as (v&?&HA); eauto using indexes_valid_weaken.
   assert (⊥ [mA; cmap_erase m]).
   { rewrite <-cmap_erase_disjoint_le; auto. }
-  destruct (HA Γ Δ'' n'' mA) as (τlr&?&?); clear HA; eauto.
+  destruct (HA Γ' Δ'' n'' mA) as (τlr&?&?); clear HA; eauto.
   destruct τlr as [|τ']; simplify_option_equality; typed_inversion_all.
   assert (mA ∪ cmap_erase m ⊆ m ∪ mf ∪ mA).
   { rewrite (sep_commutative _ mA) by auto.
@@ -316,16 +316,16 @@ Proof.
       @sep_union_subseteq_l_transitive, cmap_erase_subseteq_l. }
   assert (⊥ [mA; cmap_erase m]).
   { rewrite <-cmap_erase_disjoint_le; auto. }
-  assert ((m ∪ mf ∪ mA) !!{Γ} a = Some v).
+  assert ((m ∪ mf ∪ mA) !!{Γ'} a = Some v).
   { apply mem_lookup_subseteq with Δ'' (mA ∪ cmap_erase m); auto. }
-  assert (mem_forced Γ a (m ∪ mf ∪ mA)).
+  assert (mem_forced Γ' a (m ∪ mf ∪ mA)).
   { apply mem_forced_subseteq with Δ'' (mA ∪ cmap_erase m); eauto. }
   split; [solve_rcred|intros S' p _].
   inv_rcstep p; [inv_ehstep; simplify_equality|exfalso; eauto with cstep].
   rewrite mem_forced_force by auto.
   apply mk_ax_next with Δ'' m; simpl; auto.
   { constructor; auto. }
-  assert (✓{Γ,Δ''} (m ∪ mf ∪ mA)) by eauto.
+  assert (✓{Γ',Δ''} (m ∪ mf ∪ mA)) by eauto.
   apply ax_done; constructor; eauto using mem_lookup_typed,
     assert_weaken, indexes_valid_weaken, addr_typed_weaken.
 Qed.
@@ -349,17 +349,17 @@ Lemma ax_assign Γ δ A P1 P2 Q1 Q2 Q ass e1 e2 μ x τ :
   Γ\ δ\ A ⊨ₑ {{ P1 }} e1 {{ Q1 }} → Γ\ δ\ A ⊨ₑ {{ P2 }} e2 {{ Q2 }} →
   Γ\ δ\ A ⊨ₑ {{ P1 ★ P2 }} e1 ::={ass} e2 {{ Q }}.
 Proof.
-  intros Hx HQ Hax1 Hax2 Δ n ρ m
-    [|τ1] ?? Hlock He ??? HP; [typed_inversion_all|].
+  intros Hx HQ Hax1 Hax2 Γ' Δ n ρ m
+    [|τ1] ???? Hlock He ??? HP; [typed_inversion_all|].
   assert (Some Readable ⊆ perm_kind x)by (by transitivity (Some Writable)).
-  assert (∃ τ2, (Γ, Δ, ρ.*2) ⊢ e1 : inl τ1 ∧
-    (Γ, Δ, ρ.*2) ⊢ e2 : inr τ2 ∧ assign_typed τ1 τ2 ass)
+  assert (∃ τ2, (Γ',Δ,ρ.*2) ⊢ e1 : inl τ1 ∧
+    (Γ',Δ,ρ.*2) ⊢ e2 : inr τ2 ∧ assign_typed τ1 τ2 ass)
     as (τ2&?&?&?) by (typed_inversion_all; eauto); clear He.
   destruct HP as (m1'&m2'&Hm12&Hm12'&?&?).
   destruct (cmap_erase_union_inv m m1' m2') as (m1&m2&->&?&->&->); auto;
     simplify_mem_disjoint_hyps; clear Hm12 Hm12'.
   rewrite mem_locks_union in Hlock by auto; simpl in *; decompose_empty.
-  apply (ax_expr_compose_2 Γ δ A Q1 Q2 _ Δ (DCAssign ass) e1 e2 ρ n m1 m2
+  apply (ax_expr_compose_2 Γ' δ A Q1 Q2 _ Δ (DCAssign ass) e1 e2 ρ n m1 m2
     (inl τ1) (inr τ2)); eauto using ax_expr_funframe_weaken,
     @sep_union_subseteq_l', @sep_union_subseteq_r'.
   { esolve_elem_of. }
@@ -368,7 +368,7 @@ Proof.
     ???????????; typed_inversion_all.
   apply ax_further_alt; intros Δ'' n'' ? ff ??? Hframe;
     inversion_clear Hframe as [mA mf|]; simplify_equality.
-  destruct (HQ a' v Γ Δ' ρ n' (cmap_erase (m1' ∪ m2')))
+  destruct (HQ a' v Γ' Δ' ρ n' (cmap_erase (m1' ∪ m2')))
     as (va'&v'&(m1&m2''&?&?&(?&a&va&?&?&?&?&?)&HQ')&Hass);
     eauto 6 using indexes_valid_weaken; clear HQ.
   { rewrite cmap_erase_union.
@@ -378,13 +378,13 @@ Proof.
     as (m2&Hm&?&Hm'&->); auto; rewrite Hm in *;
     simplify_option_equality; typed_inversion_all.
   assert (TType τ = TType τ1); simplify_equality'.
-  { eapply typed_unique with (Γ,Δ') a; eauto. }
+  { eapply typed_unique with (Γ',Δ') a; eauto. }
   simplify_mem_disjoint_hyps.
-  assert (mem_writable Γ a (m1 ∪ m2 ∪ mf ∪ mA)).
+  assert (mem_writable Γ' a (m1 ∪ m2 ∪ mf ∪ mA)).
   { eapply mem_writable_subseteq with Δ'' m1;
       eauto using mem_writable_singleton,
       @sep_union_subseteq_l_transitive, @sep_union_subseteq_l'. }
-  assert (assign_sem Γ (m1 ∪ m2 ∪ mf ∪ mA) a v ass va' v').
+  assert (assign_sem Γ' (m1 ∪ m2 ∪ mf ∪ mA) a v ass va' v').
   { clear HQ'.
     assert (mA ∪ cmap_erase (m1 ∪ m2) ⊆ m1 ∪ m2 ∪ mf ∪ mA).
     { rewrite (sep_commutative _ mA) by auto.
@@ -394,7 +394,7 @@ Proof.
     { rewrite <-cmap_erase_disjoint_le; auto. }
     eapply assign_sem_subseteq with Δ'' (mA ∪ cmap_erase (m1 ∪ m2)) τ1 τ2;
       eauto 15 using addr_typed_weaken, val_typed_weaken.
-    destruct ass; destruct (Hass Γ Δ'' n'' mA) as [(?&_&?) (?&_&?)]; auto;
+    destruct ass; destruct (Hass Γ' Δ'' n'' mA) as [(?&_&?) (?&_&?)]; auto;
       clear Hass; simplify_option_equality;
       econstructor; simplify_type_equality; eauto. }
   clear Hass.
@@ -402,24 +402,24 @@ Proof.
   inv_rcstep p; [inv_ehstep; simplify_equality|exfalso; eauto 6 with cstep].
   match goal with
   | Hass : assign_sem _ ?m _ _ _ ?va'' ?v'' |- _ =>
-    destruct (assign_sem_deterministic Γ m a v ass va'' va' v'' v');
+    destruct (assign_sem_deterministic Γ' m a v ass va'' va' v'' v');
       auto; subst; clear Hass
   end.
-  assert ((Γ,Δ'') ⊢ va' : τ1 ∧ (Γ,Δ'') ⊢ v' : τ1) as [].
+  assert ((Γ',Δ'') ⊢ va' : τ1 ∧ (Γ',Δ'') ⊢ v' : τ1) as [].
   { eapply (assign_preservation _ _ (m1 ∪ m2 ∪ mf ∪ mA));
       eauto using addr_typed_weaken, val_typed_weaken. }
-  assert (⊥ [<[a:=va']{Γ}> m1; m2; mf; mA]).
+  assert (⊥ [<[a:=va']{Γ'}> m1; m2; mf; mA]).
   { by rewrite <-mem_insert_disjoint_le
       by eauto using mem_writable_singleton, addr_typed_weaken. }
-  assert (✓{Γ,Δ''} (<[a:=va']{Γ}> m1)).
+  assert (✓{Γ',Δ''} (<[a:=va']{Γ'}> m1)).
   { eauto using mem_insert_valid, mem_writable_singleton, addr_typed_weaken. }
-  assert (mem_writable Γ a (<[a:=va']{Γ}> m1)).
+  assert (mem_writable Γ' a (<[a:=va']{Γ'}> m1)).
   { eauto 6 using mem_insert_writable,
       mem_writable_singleton, addr_typed_weaken. }
-  assert (⊥ [mem_lock Γ a (<[a:=va']{Γ}> m1); m2; mf; mA]).
+  assert (⊥ [mem_lock Γ' a (<[a:=va']{Γ'}> m1); m2; mf; mA]).
   { by rewrite <-mem_lock_disjoint_le by eauto using addr_typed_weaken. }
-  assert (mem_locks (mem_lock Γ a (<[a:=va']{Γ}> m1) ∪ m2)
-    = lock_singleton Γ a ∪ mem_locks m1' ∪ mem_locks m2').
+  assert (mem_locks (mem_lock Γ' a (<[a:=va']{Γ'}> m1) ∪ m2)
+    = lock_singleton Γ' a ∪ mem_locks m1' ∪ mem_locks m2').
   { erewrite mem_locks_union, mem_locks_lock, mem_locks_insert
       by eauto using mem_writable_singleton, addr_typed_weaken.
     rewrite <-!(associative_L (∪)), <-mem_locks_union, Hm,
@@ -428,7 +428,7 @@ Proof.
   erewrite mem_insert_union, mem_lock_union
     by eauto using mem_writable_singleton, addr_typed_weaken.
   rewrite !sep_associative by auto.
-  apply mk_ax_next with Δ'' (mem_lock Γ a (<[a:=va']{Γ}> m1) ∪ m2); simpl; auto.
+  apply mk_ax_next with Δ'' (mem_lock Γ' a (<[a:=va']{Γ'}> m1) ∪ m2); simpl; auto.
   { constructor; auto. }
   { by apply reflexive_eq. } 
   { rewrite <-!sep_associative by auto; auto using mem_lock_valid. }
@@ -446,18 +446,18 @@ Lemma ax_eltl Γ δ A P Q1 Q2 e rs :
   Γ\ δ\ A ⊨ₑ {{ P }} e {{ Q1 }} →
   Γ\ δ\ A ⊨ₑ {{ P }} e %> rs {{ Q2 }}.
 Proof.
-  intros HQ Hax Δ n ρ m [σ|] ??? He ????; [|typed_inversion_all].
-  assert (∃ τ, (Γ, Δ, ρ.*2) ⊢ e : inl τ ∧ Γ ⊢ rs : τ ↣ σ) as (τ&?&?)
+  intros HQ Hax Γ' Δ n ρ m [σ|] ????? He ????; [|typed_inversion_all].
+  assert (∃ τ, (Γ',Δ,ρ.*2) ⊢ e : inl τ ∧ Γ' ⊢ rs : τ ↣ σ) as (τ&?&?)
     by (typed_inversion_all; eauto); clear He.
-  apply (ax_expr_compose_1 Γ δ A Q1 _ Δ (DCEltL rs) e ρ n m (inl τ)); auto.
+  apply (ax_expr_compose_1 Γ' δ A Q1 _ Δ (DCEltL rs) e ρ n m (inl τ)); auto.
   { esolve_elem_of. }
   clear dependent m; intros Δ' n' Ω [a|] m ??????; typed_inversion_all.
   apply ax_further_alt.
   intros Δ'' n'' ????? Hframe; inversion_clear Hframe as [mA mf|];
     simplify_equality; simplify_mem_disjoint_hyps.
-  destruct (HQ a Γ Δ' ρ n' (cmap_erase m))
+  destruct (HQ a Γ' Δ' ρ n' (cmap_erase m))
     as (a'&?&HA); eauto using indexes_valid_weaken.
-  destruct (HA Γ Δ'' n'' mA) as (τlr&?&?); clear HA; eauto.
+  destruct (HA Γ' Δ'' n'' mA) as (τlr&?&?); clear HA; eauto.
   { rewrite <-cmap_erase_disjoint_le; auto. }
   destruct τlr as [τ'|]; simplify_option_equality; typed_inversion_all.
   split; [solve_rcred|intros S' p _].
@@ -473,18 +473,18 @@ Lemma ax_eltr Γ δ A P Q1 Q2 e rs :
   Γ\ δ\ A ⊨ₑ {{ P }} e {{ Q1 }} →
   Γ\ δ\ A ⊨ₑ {{ P }} e #> rs {{ Q2 }}.
 Proof.
-  intros HQ Hax Δ n ρ m [|σ] ??? He ????; [typed_inversion_all|].
-  assert (∃ τ, (Γ, Δ, ρ.*2) ⊢ e : inr τ ∧ Γ ⊢ rs : τ ↣ σ) as (τ&?&?)
+  intros HQ Hax Γ' Δ n ρ m [|σ] ????? He ????; [typed_inversion_all|].
+  assert (∃ τ, (Γ',Δ,ρ.*2) ⊢ e : inr τ ∧ Γ' ⊢ rs : τ ↣ σ) as (τ&?&?)
     by (typed_inversion_all; eauto); clear He.
-  apply (ax_expr_compose_1 Γ δ A Q1 _ Δ (DCEltR rs) e ρ n m (inr τ)); auto.
+  apply (ax_expr_compose_1 Γ' δ A Q1 _ Δ (DCEltR rs) e ρ n m (inr τ)); auto.
   { esolve_elem_of. }
   clear dependent m; intros Δ' n' Ω [|v] m ??????; typed_inversion_all.
   apply ax_further_alt.
   intros Δ'' n'' ????? Hframe; inversion_clear Hframe as [mA mf|];
     simplify_equality; simplify_mem_disjoint_hyps.
-  destruct (HQ v Γ Δ' ρ n' (cmap_erase m))
+  destruct (HQ v Γ' Δ' ρ n' (cmap_erase m))
     as (v'&?&HA); eauto using indexes_valid_weaken.
-  destruct (HA Γ Δ'' n'' mA) as (τlr&?&?); clear HA; eauto.
+  destruct (HA Γ' Δ'' n'' mA) as (τlr&?&?); clear HA; eauto.
   { rewrite <-cmap_erase_disjoint_le; auto. }
   destruct τlr as [|τ']; simplify_option_equality; typed_inversion_all.
   split; [solve_rcred|intros S' p _].
@@ -503,15 +503,16 @@ Lemma ax_insert Γ δ A P1 P2 Q1 Q2 R e1 e2 r :
   Γ\ δ\ A ⊨ₑ {{ P2 }} e2 {{ Q2 }} →
   Γ\ δ\ A ⊨ₑ {{ P1 ★ P2 }} #[r:=e1] e2 {{ R }}.
 Proof.
-  intros HQ Hax1 Hax2 Δ n ρ m [|τ] ?? Hlocks He ??? HP; [typed_inversion_all|].
-  assert (∃ σ, (Γ, Δ, ρ.*2) ⊢ e1 : inr σ ∧
-    (Γ, Δ, ρ.*2) ⊢ e2 : inr τ ∧ Γ ⊢ r : τ ↣ σ) as (σ&?&?&?)
+  intros HQ Hax1 Hax2 Γ' Δ n ρ m [|τ] ???? Hlocks He ??? HP;
+    [typed_inversion_all|].
+  assert (∃ σ, (Γ',Δ,ρ.*2) ⊢ e1 : inr σ ∧
+    (Γ',Δ,ρ.*2) ⊢ e2 : inr τ ∧ Γ' ⊢ r : τ ↣ σ) as (σ&?&?&?)
     by (typed_inversion_all; eauto); clear He.
   destruct HP as (m1'&m2'&?&?&?&?).
   destruct (cmap_erase_union_inv m m1' m2')
     as (m1&m2&->&?&->&->); simplify_mem_disjoint_hyps; auto.
   rewrite mem_locks_union in Hlocks by auto; simpl in *; decompose_empty.
-  apply (ax_expr_compose_2 Γ δ A Q1 Q2 _ Δ (DCInsert r)
+  apply (ax_expr_compose_2 Γ' δ A Q1 Q2 _ Δ (DCInsert r)
     e1 e2 ρ n m1 m2 (inr σ) (inr τ)); eauto using ax_expr_funframe_weaken,
     @sep_union_subseteq_l', @sep_union_subseteq_r'.
   { esolve_elem_of. }
@@ -521,12 +522,12 @@ Proof.
   apply ax_further_alt.
   intros Δ'' n'' ????? Hframe; inversion_clear Hframe as [mA mf|];
     simplify_equality; simplify_mem_disjoint_hyps.
-  destruct (HQ v1 v2 Γ Δ' ρ n' (cmap_erase (m1 ∪ m2)))
+  destruct (HQ v1 v2 Γ' Δ' ρ n' (cmap_erase (m1 ∪ m2)))
     as (v'&?&HA); eauto 6 using indexes_valid_weaken.
   { rewrite cmap_erase_union.
     exists (cmap_erase m1) (cmap_erase m2); split_ands; auto.
     by rewrite <-!cmap_erase_disjoint_le. }
-  destruct (HA Γ Δ'' n'' mA) as (?&_&?); clear HA; eauto.
+  destruct (HA Γ' Δ'' n'' mA) as (?&_&?); clear HA; eauto.
   { rewrite <-cmap_erase_disjoint_le; auto. }
   simplify_option_equality; typed_inversion_all.
   split; [solve_rcred|intros S' p _].
@@ -548,15 +549,15 @@ Lemma ax_alloc Γ δ A P Q1 Q2 e τ :
   Γ\ δ\ A ⊨ₑ {{ P }} e {{ Q1 }} →
   Γ\ δ\ A ⊨ₑ {{ P }} alloc{τ} e {{ Q2 }}.
 Proof.
-  intros ? HQ Hax Δ n ρ m τlr ??? He ????.
-  assert (∃ τi, (Γ,Δ,ρ.*2) ⊢ e : inr (intT τi) ∧
-    ✓{Γ} τ ∧ τlr = inr (TType τ.*)) as (τi&?&?&->)
+  intros ? HQ Hax Γ' Δ n ρ m τlr ????? He ????.
+  assert (∃ τi, (Γ',Δ,ρ.*2) ⊢ e : inr (intT τi) ∧
+    ✓{Γ'} τ ∧ τlr = inr (TType τ.*)) as (τi&?&?&->)
     by (typed_inversion_all; eauto); clear He.
-  apply (ax_expr_compose_1 Γ δ A Q1 _ Δ
+  apply (ax_expr_compose_1 Γ' δ A Q1 _ Δ
     (DCAlloc τ) e ρ n m (inr (intT τi))); auto.
   { esolve_elem_of. }
   clear dependent m; intros Δ' n' Ω [|[vb| | | |]] m ??????; typed_inversion_all.
-  destruct (HQ (fresh ∅) vb Γ Δ' ρ n' (cmap_erase m))
+  destruct (HQ (fresh ∅) vb Γ' Δ' ρ n' (cmap_erase m))
     as (na&τi'&_&_&_&_&[[-> ?] _]&_); eauto using indexes_valid_weaken;
     typed_inversion_all.
   apply ax_further; [intros; solve_rcred|].
@@ -564,7 +565,7 @@ Proof.
     simplify_equality; simplify_mem_disjoint_hyps.
   assert (∃ o,
     S' = State [] (Expr (#{mem_locks m} ptrV (Ptr (addr_top_array o τ na))))
-      (mem_alloc Γ o true perm_full (val_new Γ (τ.[Z.to_nat na]))
+      (mem_alloc Γ' o true perm_full (val_new Γ' (τ.[Z.to_nat na]))
       (m ∪ mf ∪ mA)) ∧ o ∉ dom indexset (m ∪ mf ∪ mA))
       as (o&->&Ho); [|simplify_equality'; clear p].
   { inv_rcstep p; [inv_ehstep; by eauto|exfalso; eauto with cstep]. }
@@ -572,24 +573,24 @@ Proof.
   { rewrite mem_dom_alloc in Hdom. apply not_elem_of_dom; esolve_elem_of. }
   rewrite <-sep_associative, cmap_dom_union,
     not_elem_of_union in Ho by auto; destruct Ho.
-  assert (✓{Γ} (τ.[Z.to_nat na])) by eauto using TArray_valid.
+  assert (✓{Γ'} (τ.[Z.to_nat na])) by eauto using TArray_valid.
   assert (
-    mem_alloc Γ o true perm_full (val_new Γ (τ.[Z.to_nat na])) m ⊥ mf ∪ mA)
+    mem_alloc Γ' o true perm_full (val_new Γ' (τ.[Z.to_nat na])) m ⊥ mf ∪ mA)
     by eauto using (mem_alloc_disjoint _ Δ'); simplify_mem_disjoint_hyps.
   apply mk_ax_next with (<[o:=(τ.[Z.to_nat na],false)]>Δ'')
-    (mem_alloc Γ o true perm_full (val_new Γ (τ.[Z.to_nat na])) m);
+    (mem_alloc Γ' o true perm_full (val_new Γ' (τ.[Z.to_nat na])) m);
     eauto using mem_alloc_forward, mem_alloc_forward_least.
   { rewrite <-sep_associative, !mem_alloc_union, sep_associative by auto.
     constructor; auto. }
   { simpl. by erewrite (mem_locks_alloc _ Δ'') by eauto. }
   apply ax_done; constructor; eauto 8 using addr_top_array_typed,
     mem_alloc_index_typed, (mem_locks_alloc _ Δ'').
-  destruct (mem_alloc_singleton Γ Δ'' m o true perm_full
-    (val_new Γ (τ.[Z.to_nat na])) (τ.[Z.to_nat na]))
+  destruct (mem_alloc_singleton Γ' Δ'' m o true perm_full
+    (val_new Γ' (τ.[Z.to_nat na])) (τ.[Z.to_nat na]))
     as (m'&Hm'&?&?); auto using val_new_frozen.
   rewrite Hm' in *; simplify_mem_disjoint_hyps; clear Hm'.
   erewrite cmap_erase_union, mem_erase_singleton by eauto.
-  destruct (HQ o (intV{τi} na)%B Γ Δ' ρ n' (cmap_erase m))
+  destruct (HQ o (intV{τi} na)%B Γ' Δ' ρ n' (cmap_erase m))
     as (na'&τi''&_&m''&Hm''&?&[[? _] ->]&HQ2); eauto using indexes_valid_weaken.
   rewrite sep_left_id in Hm'' by auto; simplify_equality'.
   eapply HQ2; eauto using mem_alloc_forward, indexes_valid_weaken; clear HQ2.
@@ -597,7 +598,7 @@ Proof.
       eauto using mem_alloc_memenv_valid, mem_alloc_index_alive. }
   { eauto using mem_alloc_orig_valid. }
   { by rewrite <-cmap_erase_disjoint_le. }
-  eexists _, (addr_top o (τ.[Z.to_nat na'])), (val_new Γ (τ.[Z.to_nat na']));
+  eexists _, (addr_top o (τ.[Z.to_nat na'])), (val_new Γ' (τ.[Z.to_nat na']));
     split_ands; eauto using addr_top_typed, mem_alloc_index_typed.
 Qed.
 Lemma ax_free Γ δ A P Q1 Q2 e τ :
@@ -609,13 +610,13 @@ Lemma ax_free Γ δ A P Q1 Q2 e τ :
   Γ\ δ\ A ⊨ₑ {{ P }} e {{ Q1 }} →
   Γ\ δ\ A ⊨ₑ {{ P }} free e {{ Q2 }}.
 Proof.
-  intros HQ Hax Δ n ρ m τlr ??? He ????.
-  assert (∃ τ', (Γ,Δ,ρ.*2) ⊢ e : inl τ' ∧ τlr = inr voidT) as (τ'&?&->)
+  intros HQ Hax Γ' Δ n ρ m τlr ????? He ????.
+  assert (∃ τ', (Γ',Δ,ρ.*2) ⊢ e : inl τ' ∧ τlr = inr voidT) as (τ'&?&->)
     by (typed_inversion_all; eauto); clear He.
-  apply (ax_expr_compose_1 Γ δ A Q1 _ Δ DCFree e ρ n m (inl τ')); auto.
+  apply (ax_expr_compose_1 Γ' δ A Q1 _ Δ DCFree e ρ n m (inl τ')); auto.
   { esolve_elem_of. }
   clear dependent m; intros Δ' n' Ω [a|] m ??????; typed_inversion_all.
-  destruct (HQ a Γ Δ' ρ n' (cmap_erase m))
+  destruct (HQ a Γ' Δ' ρ n' (cmap_erase m))
     as (na&?&?&Hm'&?&[Ha' ->]&m1&m2'&?&?&(ν&a'&v&_&?&?&?&?)&?);
     eauto using indexes_valid_weaken.
   rewrite sep_left_id in Hm' by auto;
@@ -656,18 +657,18 @@ Lemma ax_unop Γ δ A P Q1 Q2 op e :
   Γ\ δ\ A ⊨ₑ {{ P }} e {{ Q1 }} →
   Γ\ δ\ A ⊨ₑ {{ P }} @{op} e {{ Q2 }}.
 Proof.
-  intros HQ Hax Δ n ρ m [|σ] ??? He ?? HA HP; [typed_inversion_all|].
-  assert (∃ τ, (Γ, Δ, ρ.*2) ⊢ e : inr τ ∧ unop_typed op τ σ)
+  intros HQ Hax Γ' Δ n ρ m [|σ] ????? He ?? HA HP; [typed_inversion_all|].
+  assert (∃ τ, (Γ',Δ,ρ.*2) ⊢ e : inr τ ∧ unop_typed op τ σ)
     as (τ&?&?) by (typed_inversion_all; eauto); clear He.
-  apply (ax_expr_compose_1 Γ δ A Q1 _ Δ (DCUnOp op) e ρ n m (inr τ)); auto.
+  apply (ax_expr_compose_1 Γ' δ A Q1 _ Δ (DCUnOp op) e ρ n m (inr τ)); auto.
   { esolve_elem_of. }
   clear dependent m. intros Δ' n' Ω [a|] m ??????; typed_inversion_all.
   apply ax_further_alt.
   intros Δ'' n'' ????? Hframe; inversion_clear Hframe as [mA mf|];
     simplify_equality; simplify_mem_disjoint_hyps.
-  destruct (HQ v Γ Δ' ρ n' (cmap_erase m))
+  destruct (HQ v Γ' Δ' ρ n' (cmap_erase m))
     as (v'&?&HA); eauto using indexes_valid_weaken.
-  destruct (HA Γ Δ'' n'' mA) as (?&_&?); clear HA; eauto.
+  destruct (HA Γ' Δ'' n'' mA) as (?&_&?); clear HA; eauto.
   { rewrite <-cmap_erase_disjoint_le; auto. }
   simplify_option_equality.
   assert (val_unop_ok (m ∪ mf ∪ mA) op v).
@@ -691,15 +692,16 @@ Lemma ax_binop Γ δ A P1 P2 Q1 Q2 R op e1 e2 :
   Γ\ δ\ A ⊨ₑ {{ P2 }} e2 {{ Q2 }} →
   Γ\ δ\ A ⊨ₑ {{ P1 ★ P2 }} e1 @{op} e2 {{ R }}.
 Proof.
-  intros HQ Hax1 Hax2 Δ n ρ m [|σ] ?? Hlock He ?? HA HP; [typed_inversion_all|].
-  assert (∃ τ1 τ2, (Γ, Δ, ρ.*2) ⊢ e1 : inr τ1 ∧
-    (Γ, Δ, ρ.*2) ⊢ e2 : inr τ2 ∧ binop_typed op τ1 τ2 σ)
+  intros HQ Hax1 Hax2 Γ' Δ n ρ m [|σ] ???? Hlock He ?? HA HP;
+    [typed_inversion_all|].
+  assert (∃ τ1 τ2, (Γ',Δ,ρ.*2) ⊢ e1 : inr τ1 ∧
+    (Γ',Δ,ρ.*2) ⊢ e2 : inr τ2 ∧ binop_typed op τ1 τ2 σ)
     as (τ1&τ2&?&?&?) by (typed_inversion_all; eauto); clear He.
   destruct HP as (m1'&m2'&?&?&?&?).
   destruct (cmap_erase_union_inv m m1' m2')
     as (m1&m2&->&?&->&->); simplify_mem_disjoint_hyps; auto.
   rewrite mem_locks_union in Hlock by auto; simpl in *; decompose_empty.
-  apply (ax_expr_compose_2 Γ δ A Q1 Q2 _ Δ (DCBinOp op) e1 e2 ρ n m1 m2
+  apply (ax_expr_compose_2 Γ' δ A Q1 Q2 _ Δ (DCBinOp op) e1 e2 ρ n m1 m2
     (inr τ1) (inr τ2)); eauto using ax_expr_funframe_weaken,
     @sep_union_subseteq_l', @sep_union_subseteq_r'.
   { esolve_elem_of. }
@@ -709,17 +711,17 @@ Proof.
   apply ax_further_alt.
   intros Δ'' n'' ????? Hframe; inversion_clear Hframe as [mA mf|];
     simplify_equality; simplify_mem_disjoint_hyps.
-  destruct (HQ v1 v2 Γ Δ' ρ n' (cmap_erase (m1 ∪ m2)))
+  destruct (HQ v1 v2 Γ' Δ' ρ n' (cmap_erase (m1 ∪ m2)))
     as (v'&?&HA); eauto 6 using indexes_valid_weaken.
   { rewrite cmap_erase_union.
     exists (cmap_erase m1) (cmap_erase m2); split_ands; auto.
     by rewrite <-!cmap_erase_disjoint_le. }
-  destruct (HA Γ Δ'' n'' mA) as (?&_&?); clear HA; eauto.
+  destruct (HA Γ' Δ'' n'' mA) as (?&_&?); clear HA; eauto.
   { rewrite <-cmap_erase_disjoint_le; auto. }
   simplify_option_equality.
-  assert (val_binop_ok Γ (m1 ∪ m2 ∪ mf ∪ mA) op v1 v2).
+  assert (val_binop_ok Γ' (m1 ∪ m2 ∪ mf ∪ mA) op v1 v2).
   { eapply val_binop_ok_weaken
-      with Γ Δ' (mA ∪ cmap_erase (m1 ∪ m2)) τ1 τ2; eauto.
+      with Γ' Δ' (mA ∪ cmap_erase (m1 ∪ m2)) τ1 τ2; eauto.
     intros; eapply cmap_subseteq_index_alive; eauto.
     rewrite (sep_commutative _ mA) by auto.
     apply sep_preserving_l; auto using
@@ -737,22 +739,22 @@ Lemma ax_cast Γ δ A P Q1 Q2 σ e :
   Γ\ δ\ A ⊨ₑ {{ P }} e {{ Q1 }} →
   Γ\ δ\ A ⊨ₑ {{ P }} cast{σ} e {{ Q2 }}.
 Proof.
-  intros HQ Hax Δ n ρ m [|σ'] ??? He ?? HA HP; [typed_inversion_all|].
-  assert (∃ τ, (Γ, Δ, ρ.*2) ⊢ e : inr τ ∧ cast_typed τ σ ∧ ✓{Γ} σ ∧ σ' = σ)
+  intros HQ Hax Γ' Δ n ρ m [|σ'] ????? He ?? HA HP; [typed_inversion_all|].
+  assert (∃ τ, (Γ',Δ,ρ.*2) ⊢ e : inr τ ∧ cast_typed τ σ ∧ ✓{Γ'} σ ∧ σ' = σ)
     as (τ&?&?&?&->) by (typed_inversion_all; eauto); clear He.
-  apply (ax_expr_compose_1 Γ δ A Q1 _ Δ (DCCast σ) e ρ n m (inr τ)); auto.
+  apply (ax_expr_compose_1 Γ' δ A Q1 _ Δ (DCCast σ) e ρ n m (inr τ)); auto.
   { esolve_elem_of. }
   clear dependent m. intros Δ' n' Ω [a|] m ??????; typed_inversion_all.
   apply ax_further_alt.
   intros Δ'' n'' ????? Hframe; inversion_clear Hframe as [mA mf|];
     simplify_equality; simplify_mem_disjoint_hyps.
-  destruct (HQ v Γ Δ' ρ n' (cmap_erase m))
+  destruct (HQ v Γ' Δ' ρ n' (cmap_erase m))
     as (v'&?&HA); eauto using indexes_valid_weaken.
-  destruct (HA Γ Δ'' n'' mA) as (?&_&?); clear HA; eauto.
+  destruct (HA Γ' Δ'' n'' mA) as (?&_&?); clear HA; eauto.
   { rewrite <-cmap_erase_disjoint_le; auto. }
   simplify_option_equality.
-  assert (val_cast_ok Γ (m ∪ mf ∪ mA) (TType σ) v).
-  { eapply val_cast_ok_weaken with Γ Δ' (mA ∪ cmap_erase m) τ; eauto.
+  assert (val_cast_ok Γ' (m ∪ mf ∪ mA) (TType σ) v).
+  { eapply val_cast_ok_weaken with Γ' Δ' (mA ∪ cmap_erase m) τ; eauto.
     intros; eapply cmap_subseteq_index_alive; eauto.
     rewrite (sep_commutative _ mA) by auto.
     apply sep_preserving_l; auto using
@@ -772,12 +774,12 @@ Lemma ax_expr_if Γ δ A P P' P1 P2 Q e e1 e2 :
   Γ\ δ\ A ⊨ₑ {{ P1 }} e1 {{ Q }} → Γ\ δ\ A ⊨ₑ {{ P2 }} e2 {{ Q }} →
   Γ\ δ\ A ⊨ₑ {{ P }} if{e} e1 else e2 {{ Q }}.
 Proof.
-  intros HP' HP1 HP2 Hax Hax1 Hax2 Δ n ρ m τlr ??? He ????;
+  intros HP' HP1 HP2 Hax Hax1 Hax2 Γ' Δ n ρ m τlr ????? He ????;
     simpl in *; decompose_empty.
-  assert (∃ τb, (Γ,Δ,ρ.*2) ⊢ e : inr (baseT τb) ∧ τb ≠ voidT%BT ∧
-    (Γ,Δ,ρ.*2) ⊢ e1 : τlr ∧ (Γ,Δ,ρ.*2) ⊢ e2 : τlr)
+  assert (∃ τb, (Γ',Δ,ρ.*2) ⊢ e : inr (baseT τb) ∧ τb ≠ voidT%BT ∧
+    (Γ',Δ,ρ.*2) ⊢ e1 : τlr ∧ (Γ',Δ,ρ.*2) ⊢ e2 : τlr)
     as (τb&?&?&?&?) by (typed_inversion_all; eauto); clear He.
-  apply (ax_expr_compose_1 Γ δ A
+  apply (ax_expr_compose_1 Γ' δ A
     P' _ Δ (DCIf e1 e2) e ρ n m (inr (baseT τb))); auto.
   { esolve_elem_of. }
   { esolve_elem_of. }
@@ -789,7 +791,7 @@ Proof.
   assert (base_val_branchable (m ∪ mf ∪ mA) vb).
   { assert (⊥ [cmap_erase m; mf; mA])
       by (rewrite <-cmap_erase_disjoint_le; auto).
-    destruct (HP' vb Γ Δ'' ρ n'' (mA ∪ cmap_erase m)) as (?&?&?&?);
+    destruct (HP' vb Γ' Δ'' ρ n'' (mA ∪ cmap_erase m)) as (?&?&?&?);
       simpl; eauto using indexes_valid_weaken.
     { exists mA (cmap_erase m); split_ands; auto.
       eauto using assert_weaken, indexes_valid_weaken. }
@@ -812,7 +814,7 @@ Proof.
     { eauto using mem_unlock_all_valid. }
     apply Hax1; rewrite ?mem_erase_unlock_all;
       eauto 8 using mem_unlock_all_valid, indexes_valid_weaken,
-      mem_locks_unlock_all, expr_typed_weaken.
+      mem_locks_unlock_all, expr_typed_weaken, funenv_valid_weaken.
     + exists mA; split_ands; eauto.
     + eapply HP1; eauto using indexes_valid_weaken, assert_weaken.
   * rewrite !mem_unlock_union, <-mem_unlock_all_spec
@@ -823,7 +825,7 @@ Proof.
     { eauto using mem_unlock_all_valid. }
     apply Hax2; rewrite ?mem_erase_unlock_all;
       eauto 8 using mem_unlock_all_valid, indexes_valid_weaken,
-      mem_locks_unlock_all, expr_typed_weaken.
+      mem_locks_unlock_all, expr_typed_weaken, funenv_valid_weaken.
     + exists mA; split_ands; eauto.
     + eapply HP2; eauto using indexes_valid_weaken, assert_weaken.
   * destruct (decide (base_val_is_0 vb)); exfalso; eauto with cstep.
@@ -833,11 +835,11 @@ Lemma ax_expr_comma Γ δ A P P' Q e1 e2 :
   Γ\ δ\ A ⊨ₑ {{ P' }} e2 {{ Q }} →
   Γ\ δ\ A ⊨ₑ {{ P }} e1 ,, e2 {{ Q }}.
 Proof.
-  intros Hax1 Hax2 Δ n ρ m τlr2 ??? He1e2 He ???.
-  assert (∃ τlr1, (Γ, Δ, ρ.*2) ⊢ e1 : τlr1 ∧ (Γ, Δ, ρ.*2) ⊢ e2 : τlr2)
+  intros Hax1 Hax2 Γ' Δ n ρ m τlr2 ????? He1e2 He ???.
+  assert (∃ τlr1, (Γ',Δ,ρ.*2) ⊢ e1 : τlr1 ∧ (Γ',Δ,ρ.*2) ⊢ e2 : τlr2)
     as (τlr1&?&?) by (typed_inversion_all; eauto); clear He1e2.
   simpl in He; decompose_empty.
-  apply (ax_expr_compose_1 Γ δ A
+  apply (ax_expr_compose_1 Γ' δ A
     (λ _, P' ◊)%A _ Δ (DCComma e2) e1 ρ n m τlr1); auto.
   { esolve_elem_of. }
   clear dependent m; intros Δ' n' Ω ν m ??????; simplify_equality'.
@@ -855,7 +857,7 @@ Proof.
   { eauto using mem_unlock_all_valid. }
   apply Hax2; rewrite ?mem_erase_unlock_all;
     eauto 7 using mem_unlock_all_valid, indexes_valid_weaken,
-    mem_locks_unlock_all, expr_typed_weaken, assert_weaken.
+    mem_locks_unlock_all, expr_typed_weaken, assert_weaken, funenv_valid_weaken.
   exists mA; split_ands; eauto.
 Qed.
 End axiomatic_expressions.
